pulse/share/steel/examples/pulse/by-example/PulseTutorial.Algorithms.fst
@@ -1,3 +1,19 @@
+(*
+   Copyright 2023 Microsoft Research
+
+   Licensed under the Apache License, Version 2.0 (the "License");
+   you may not use this file except in compliance with the License.
+   You may obtain a copy of the License at
+
+       http://www.apache.org/licenses/LICENSE-2.0
+
+   Unless required by applicable law or agreed to in writing, software
+   distributed under the License is distributed on an "AS IS" BASIS,
+   WITHOUT WARRANTIES OR CONDITIONS OF ANY KIND, either express or implied.
+   See the License for the specific language governing permissions and
+   limitations under the License.
+*)
+
 module PulseTutorial.Algorithms
 
 open FStar.Mul
@@ -6,11 +22,17 @@ open FStar.SizeT
 open Pulse.Lib.Pervasives
 open Pulse.Lib.Array
 
-module R = Pulse.Lib.Reference
 module SZ = FStar.SizeT
+module G = FStar.Ghost
+module R = Pulse.Lib.Reference
 
-let count (#a:eqtype) (x:a) (s:Seq.seq a) (j:nat { j <= Seq.length s }) =
+let count (#a:eqtype) (x:a) (s:Seq.seq a) (j:nat { j <= Seq.length s }) : GTot nat =
   Seq.count x (Seq.slice s 0 j)
+
+let count_len (#a:eqtype) (x:a) (s:Seq.seq a) (j:nat { j <= Seq.length s })
+  : Lemma (ensures count x s j <= j)
+          [SMTPat (count x s j)] =
+  admit ()
 
 let count_next (#a:eqtype) (x:a) (s:Seq.seq a) (j:nat { j < Seq.length s })
   : Lemma
@@ -21,16 +43,17 @@ let count_next (#a:eqtype) (x:a) (s:Seq.seq a) (j:nat { j < Seq.length s })
   assert (Seq.equal (Seq.slice s 0 (j + 1)) (Seq.append s_0_j sj));
   Seq.lemma_append_count s_0_j sj
 
+#push-options "--z3rlimit_factor 2"
 ```pulse
-fn majority (#a:eqtype) #p (#s:Seq.seq a) (votes:array a) (len:SZ.t { SZ.v len == Seq.length s })
-  requires pts_to votes #p s ** pure (SZ.v len > 0)
+fn majority (#a:eqtype) #p (#s:G.erased _) (votes:array a) (len:SZ.t { SZ.v len == Seq.length s })
+  requires pts_to votes #p s ** pure (0 < SZ.v len /\ SZ.fits (2 * SZ.v len))
   returns x:option a
   ensures pts_to votes #p s **
           pure ((x == None ==> (forall (y:a). 2 * count y s (SZ.v len) <= SZ.v len)) /\
                 (Some? x ==> SZ.v len < 2 * count (Some?.v x) s (SZ.v len)))
 {
   let mut i = 1sz;
-  let mut k = 1;
+  let mut k = 1sz;
   let votes_0 = votes.(0sz);
   let mut cand = votes_0;
   assert (pure (count votes_0 s 1 == 1));
@@ -46,9 +69,9 @@ fn majority (#a:eqtype) #p (#s:Seq.seq a) (votes:array a) (len:SZ.t { SZ.v len =
        R.pts_to cand vcand **
        pure (
          SZ.v vi <= Seq.length s /\
-         0 <= vk /\ vk <= count vcand s (SZ.v vi) /\
-         2 * (count vcand s (SZ.v vi) - vk) <= SZ.v vi - vk /\
-         (forall (vcand':a). vcand' =!= vcand ==> 2 * count vcand' s (SZ.v vi) <= SZ.v vi - vk) /\
+         0 <= SZ.v vk /\ SZ.v vk <= count vcand s (SZ.v vi) /\
+         2 * (count vcand s (SZ.v vi) - SZ.v vk) <= SZ.v vi - SZ.v vk /\
+         (forall (vcand':a). vcand' =!= vcand ==> 2 * count vcand' s (SZ.v vi) <= SZ.v vi - SZ.v vk) /\
          b == (SZ.v vi < SZ.v len)))
   {
     let vi = !i;
@@ -56,28 +79,28 @@ fn majority (#a:eqtype) #p (#s:Seq.seq a) (votes:array a) (len:SZ.t { SZ.v len =
     let vcand = !cand;
     let votes_i = votes.(vi);
     count_next vcand s (SZ.v vi);
-    if (vk = 0) {
+    if (vk = 0sz) {
       cand := votes_i;
-      k := 1;
+      k := 1sz;
       i := vi +^ 1sz
     } else if (votes_i = vcand) {
-      k := vk + 1;
+      k := vk +^ 1sz;
       i := vi +^ 1sz
     } else {
-      k := vk - 1;
+      k := vk -^ 1sz;
       i := vi +^ 1sz
     }
   };
 
   let vk = !k;
   let vcand = !cand;
-  if (vk = 0) {
+  if (vk = 0sz) {
     None #a
-  } else if (SZ.v len < 2 * vk) {
+  } else if (len <^ 2sz *^ vk) {
     Some vcand
   } else {
     i := 0sz;
-    k := 0;
+    k := 0sz;
     while (
       let vi = !i;
       (vi <^ len)
@@ -88,7 +111,7 @@ fn majority (#a:eqtype) #p (#s:Seq.seq a) (votes:array a) (len:SZ.t { SZ.v len =
          R.pts_to i vi **
          R.pts_to k vk **
          pure (SZ.v vi <= Seq.length s /\
-               vk == count vcand s (SZ.v vi) /\
+               SZ.v vk == count vcand s (SZ.v vi) /\
                b == (SZ.v vi < SZ.v len)))
     {
       let vi = !i;
@@ -96,7 +119,7 @@ fn majority (#a:eqtype) #p (#s:Seq.seq a) (votes:array a) (len:SZ.t { SZ.v len =
       let votes_i = votes.(vi);
       count_next vcand s (SZ.v vi);
       if (votes_i = vcand) {
-        k := vk + 1;
+        k := vk +^ 1sz;
         i := vi +^ 1sz
       } else {
         i := vi +^ 1sz
@@ -104,7 +127,7 @@ fn majority (#a:eqtype) #p (#s:Seq.seq a) (votes:array a) (len:SZ.t { SZ.v len =
     };
 
     let vk = !k;
-    if (SZ.v len < 2 * vk) {
+    if (len <^ 2sz *^ vk) {
       Some vcand
     } else {
       None #a
@@ -112,3 +135,4 @@ fn majority (#a:eqtype) #p (#s:Seq.seq a) (votes:array a) (len:SZ.t { SZ.v len =
   }
 }
 ```
+#pop-options
